Chapter 5.3 (3)

chapter05.v
@@ -270,3 +270,55 @@ Section evalCmd_coind.
     destruct (WhileCase H) as [[? ?] | [? [? [? ?]]]]; subst; econstructor; eauto.
   Qed.
 End evalCmd_coind.
+
+Fixpoint optExp (e : exp) : exp :=
+  match e with
+  | Plus (Const 0) e => optExp e
+  | Plus e1 e2 => Plus (optExp e1) (optExp e2)
+  | _ => e
+  end
+.
+
+Fixpoint optCmd (c : cmd) : cmd :=
+  match c with
+  | Assign v e => Assign v (optExp e)
+  | Seq c1 c2 => Seq (optCmd c1) (optCmd c2)
+  | While e c => While (optExp e) (optCmd c)
+  end
+.
+
+Lemma optExp_correct : forall vs e ,
+    evalExp vs (optExp e) = evalExp vs e.
+      induction e; crush;
+      repeat (match goal with
+              | [ |- context[match ?E with Const _ => _ | _ => _ end]] => destruct E
+              | [ |- context [match ?E with O => _ | S _ => _ end ]] => destruct E
+              end; crush).
+Qed.
+
+Hint Rewrite optExp_correct.
+
+Ltac finisher :=
+  match goal with
+  | [ H : evalCmd _ _ _ |- _ ] => ((inversion H; [])
+                                   || (inversion H; [|])); subst
+  end; crush; eauto 10.
+
+Lemma optCmd_correct1 : forall vs1 c vs2 ,
+    evalCmd vs1 c vs2 -> evalCmd vs1 (optCmd c) vs2.
+      intros; apply (evalCmd_coind (fun vs1 c' vs2 => exists c , evalCmd vs1 c vs2 /\ c' = optCmd c)); eauto; crush; match goal with
+  | [ H : _ = optCmd ?E |- _ ] => destruct E; simpl in *; discriminate || injection H; intros; subst
+                                                                                                                     end; finisher.
+Qed.
+
+Lemma optCmd_correct2 : forall vs1 c vs2 ,
+    evalCmd vs1 (optCmd c) vs2 -> evalCmd vs1 c vs2.
+      intros; apply (evalCmd_coind (fun vs1 c vs2 => evalCmd vs1 (optCmd c) vs2));
+      crush; finisher.
+Qed.
+
+Theorem optCmd_correct : forall vs1 c vs2 ,
+    evalCmd vs1 (optCmd c) vs2 <-> evalCmd vs1 c vs2.
+      intuition; apply optCmd_correct1
+                 || apply optCmd_correct2; assumption.
+Qed.
